WIP: Start to prove ExpressionToSexpr

Source/DafnyCore/Backends/SExpression/DafnyToSExpressionCompiler.dfy
@@ -18,9 +18,9 @@ module {:extern} DafnyToSExpressionCompiler {
     decreases mod, 1
   {
     StringSeqToSexpr(["Module.Module",
-                        NameToSexpr(mod.name),
-                        MapJoin(AttributeToSexpr, mod.attributes),
-                        OptionToSexpr(mod.body, x => MapJoin(i => ModuleItemToSexpr(mod, i), x))])
+                      NameToSexpr(mod.name),
+                      MapJoin(AttributeToSexpr, mod.attributes),
+                      OptionToSexpr(mod.body, x => MapJoin(i => ModuleItemToSexpr(mod, i), x))])
   }
 
   function NameToSexpr(name: DAST.Name): string {
@@ -36,10 +36,10 @@ module {:extern} DafnyToSExpressionCompiler {
   {
     match modItem
     case Module(mod) =>
-      // TODO: Move this as a precondition and prove it at call sites
+      // TODO: Move this to a precondition and prove it at call sites
       assume {:axiom} mod < parent;
       StringSeqToSexpr(["ModuleItem.Module", ModuleToSexpr(mod)])
-    case Class(cls) => StringSeqToSexpr(["ModuleItem.Class", ClassToSexpr(cls)]) 
+    case Class(cls) => StringSeqToSexpr(["ModuleItem.Class", ClassToSexpr(cls)])
     case Trait(trt) => StringSeqToSexpr(["ModuleItem.Trait", TraitToSexpr(trt)])
     case Newtype(nt) => StringSeqToSexpr(["ModuleItem.Newtype", NewtypeToSexpr(nt)])
     case Datatype(dt) => StringSeqToSexpr(["ModuleItem.Datatype", DatatypeToSexpr(dt)])
@@ -47,54 +47,54 @@ module {:extern} DafnyToSExpressionCompiler {
 
   function ClassToSexpr(cls: DAST.Class): string {
     StringSeqToSexpr(["Class.Class",
-                        NameToSexpr(cls.name),
-                        IdentToSexpr(cls.enclosingModule),
-                        MapJoin(TypeArgDeclToSexpr, cls.typeParams),
-                        MapJoin(TypeToSexpr, cls.superClasses),
-                        MapJoin(FieldToSexpr, cls.fields),
-                        MapJoin(ClassItemToSexpr, cls.body),
-                        MapJoin(AttributeToSexpr, cls.attributes)])
+                      NameToSexpr(cls.name),
+                      IdentToSexpr(cls.enclosingModule),
+                      MapJoin(TypeArgDeclToSexpr, cls.typeParams),
+                      MapJoin(TypeToSexpr, cls.superClasses),
+                      MapJoin(FieldToSexpr, cls.fields),
+                      MapJoin(ClassItemToSexpr, cls.body),
+                      MapJoin(AttributeToSexpr, cls.attributes)])
   }
 
   function TraitToSexpr(trt: DAST.Trait): string {
     StringSeqToSexpr(["Trait.Trait",
-                        NameToSexpr(trt.name),
-                        MapJoin(TypeArgDeclToSexpr, trt.typeParams),
-                        MapJoin(ClassItemToSexpr, trt.body),
-                        MapJoin(AttributeToSexpr, trt.attributes)])
+                      NameToSexpr(trt.name),
+                      MapJoin(TypeArgDeclToSexpr, trt.typeParams),
+                      MapJoin(ClassItemToSexpr, trt.body),
+                      MapJoin(AttributeToSexpr, trt.attributes)])
   }
 
   function NewtypeToSexpr(nt: DAST.Newtype): string {
     StringSeqToSexpr(["Newtype.Newtype",
-                        NameToSexpr(nt.name),
-                        MapJoin(TypeArgDeclToSexpr, nt.typeParams),
-                        TypeToSexpr(nt.base),
-                        NewtypeRangeToSexpr(nt.range),
-                        MapJoin(StatementToSexpr, nt.witnessStmts),
-                        OptionToSexpr(nt.witnessExpr, ExpressionToSexpr),
-                        MapJoin(AttributeToSexpr, nt.attributes)])
+                      NameToSexpr(nt.name),
+                      MapJoin(TypeArgDeclToSexpr, nt.typeParams),
+                      TypeToSexpr(nt.base),
+                      NewtypeRangeToSexpr(nt.range),
+                      MapJoin(StatementToSexpr, nt.witnessStmts),
+                      OptionToSexpr(nt.witnessExpr, ExpressionToSexpr),
+                      MapJoin(AttributeToSexpr, nt.attributes)])
   }
 
   function DatatypeToSexpr(dt: DAST.Datatype): string {
     StringSeqToSexpr(["Datatype.Datatype",
-                        NameToSexpr(dt.name),
-                        IdentToSexpr(dt.enclosingModule),
-                        MapJoin(TypeArgDeclToSexpr, dt.typeParams),
-                        MapJoin(DatatypeCtorToSexpr, dt.ctors),
-                        MapJoin(ClassItemToSexpr, dt.body),
-                        Std.Strings.OfBool(dt.isCo),
-                        MapJoin(AttributeToSexpr, dt.attributes)])
+                      NameToSexpr(dt.name),
+                      IdentToSexpr(dt.enclosingModule),
+                      MapJoin(TypeArgDeclToSexpr, dt.typeParams),
+                      MapJoin(DatatypeCtorToSexpr, dt.ctors),
+                      MapJoin(ClassItemToSexpr, dt.body),
+                      Std.Strings.OfBool(dt.isCo),
+                      MapJoin(AttributeToSexpr, dt.attributes)])
   }
 
   function IdentToSexpr(ident: DAST.Ident): string {
     StringSeqToSexpr(["Ident.Ident",
-                        NameToSexpr(ident.id)])
+                      NameToSexpr(ident.id)])
   }
 
   function TypeArgDeclToSexpr(typeArgDecl: DAST.TypeArgDecl): string {
     StringSeqToSexpr(["TypeArgDecl.TypeArgDecl",
-                        IdentToSexpr(typeArgDecl.name),
-                        MapJoin(TypeArgBoundToSexpr, typeArgDecl.bounds)])
+                      IdentToSexpr(typeArgDecl.name),
+                      MapJoin(TypeArgBoundToSexpr, typeArgDecl.bounds)])
   }
 
   function TypeToSexpr(t: DAST.Type): string
@@ -103,40 +103,164 @@ module {:extern} DafnyToSExpressionCompiler {
     match t
     case Path(ids, typeArgs, resolved) =>
       StringSeqToSexpr(["Type.Path",
-                          MapJoin(IdentToSexpr, ids),
-                          MapJoin((x) requires x in typeArgs => (TypeToSexpr(x)),
-                                  typeArgs),
-                          ResolvedTypeToSexpr(resolved)])
-    case Nullable(t') => "Type.Nullable: TODO"
-    case Tuple(ts) => "Type.Tuple: TODO"
-    case Array(element, dims) => "Type. Array: TODO"
+                        MapJoin(IdentToSexpr, ids),
+                        MapJoinTypeToSexpr(typeArgs),
+                        ResolvedTypeToSexpr(resolved)])
+    case Nullable(t') =>
+      StringSeqToSexpr(["Type.Nullable",
+                        TypeToSexpr(t')])
+    case Tuple(ts) =>
+      StringSeqToSexpr(["Type.Tuple",
+                        MapJoinTypeToSexpr(ts)])
+    case Array(element, dims) =>
+      StringSeqToSexpr(["Type.Array",
+                        TypeToSexpr(element),
+                        Std.Strings.OfNat(dims)])
     case Seq(element) =>
-      StringSeqToSexpr(["Type.Seq", TypeToSexpr(element)])
-    case Set(element) => "Type.Set: TODO"
-    case Multiset(element) => "Type.Multiset: TODO"
-    case Map(key, value) => "Type.Map: TODO"
-    case SetBuilder(element) => "Type.SetBuilder: TODO"
-    case MapBuilder(key, value) => "Type.MapBuilder: TODO"
-    case Arrow(args, result) => "Type.Arrow: TODO"
-    case Primitive(primitive) => "Type.Primitive: TODO"
-    case Passthrough(str) => "Type.Passthrough: TODO"
-    case TypeArg(id) => "Type.TypeArg: TODO"
+      StringSeqToSexpr(["Type.Seq",
+                        TypeToSexpr(element)])
+    case Set(element) =>
+      StringSeqToSexpr(["Type.Set",
+                        TypeToSexpr(element)])
+    case Multiset(element) =>
+      StringSeqToSexpr(["Type.Multiset",
+                        TypeToSexpr(element)])
+    case Map(key, value) =>
+      StringSeqToSexpr(["Type.Map",
+                        TypeToSexpr(key),
+                        TypeToSexpr(value)])
+    case SetBuilder(element) =>
+      StringSeqToSexpr(["Type.SetBuilder",
+                        TypeToSexpr(element)])
+    case MapBuilder(key, value) =>
+      StringSeqToSexpr(["Type.MapBuilder",
+                        TypeToSexpr(key),
+                        TypeToSexpr(value)])
+    case Arrow(args, result) =>
+      StringSeqToSexpr(["Type.Arrow",
+                        MapJoinTypeToSexpr(args),
+                        TypeToSexpr(result)])
+    case Primitive(primitive) =>
+      StringSeqToSexpr(["Type.Primitive",
+                        PrimitiveToSexpr(primitive)])
+    case Passthrough(str) =>
+      StringSeqToSexpr(["Type.Passthrough",
+                        str])
+    case TypeArg(id) =>
+      StringSeqToSexpr(["Type.TypeArg",
+                        IdentToSexpr(id)])
+  }
+
+  // eta-expansion required; cannot be made generic
+  function MapJoinTypeToSexpr(ts: seq<DAST.Type>): string
+  {
+    // need precondition to prove termination in TypeToSexpr
+    MapJoin((x) requires x in ts => (TypeToSexpr(x)), ts)
   }
 
   function FieldToSexpr(field: DAST.Field): string {
-    "FieldToSexpr: TODO"
+    StringSeqToSexpr(["Field.Field",
+                      FormalToSexpr(field.formal),
+                      OptionToSexpr(field.defaultValue, ExpressionToSexpr)])
   }
 
   function ClassItemToSexpr(classItem: DAST.ClassItem): string {
-    "ClassItemToSexpr: TODO"
+    // Need to use match here since classItem.m is not defined
+    match classItem
+    case Method(m) =>
+      StringSeqToSexpr(["ClassItem.Method",
+                        MethodToSexpr(m)])
   }
 
   function NewtypeRangeToSexpr(range: DAST.NewtypeRange): string {
-    "NewtypeRangeToSexpr: TODO"
+    match range
+    case U8 => StringSeqToSexpr(["NewtypeRange.U8"])
+    case I8 => StringSeqToSexpr(["NewtypeRange.I8"])
+    case U16 => StringSeqToSexpr(["NewtypeRange.U16"])
+    case I16 => StringSeqToSexpr(["NewtypeRange.I16"])
+    case U32 => StringSeqToSexpr(["NewtypeRange.U32"])
+    case I32 => StringSeqToSexpr(["NewtypeRange.I32"])
+    case U64 => StringSeqToSexpr(["NewtypeRange.U64"])
+    case I64 => StringSeqToSexpr(["NewtypeRange.I64"])
+    case U128 => StringSeqToSexpr(["NewtypeRange.U128"])
+    case I128 => StringSeqToSexpr(["NewtypeRange.I128"])
+    case BigInt => StringSeqToSexpr(["NewtypeRange.BigInt"])
+    case NoRange => StringSeqToSexpr(["NewtypeRange.NoRange"])
   }
 
-  function ExpressionToSexpr(expr: DAST.Expression): string {
-    "ExpressionToSexpr: TODO"
+  function ExpressionToSexpr(expr: DAST.Expression): string
+    decreases expr
+  {
+    match expr
+    case Literal(literal) =>
+      StringSeqToSexpr(["Expression.Literal",
+                        LiteralToSexpr(literal)])
+    case Ident(name) =>
+      StringSeqToSexpr(["Expression.Ident",
+                        NameToSexpr(name)])
+    case Companion(ids) =>
+      StringSeqToSexpr(["Expression.Companion",
+                        MapJoin(IdentToSexpr, ids)])
+    case Tuple(exprs) =>
+      StringSeqToSexpr(["Expression.Tuple",
+                        MapJoinExpressionToSexpr(exprs)])
+    case New(path, typeArgs, args) =>
+      StringSeqToSexpr(["Expression.New",
+                        MapJoin(IdentToSexpr, path),
+                        MapJoin(TypeToSexpr, typeArgs),
+                        MapJoinExpressionToSexpr(args)])
+    case NewArray(dims, typ) =>
+      StringSeqToSexpr(["Expression.NewArray",
+                          MapJoinExpressionToSexpr(dims),
+                          TypeToSexpr(typ)])
+    case DatatypeValue(datatypeType, typeArgs, variant, isCo, contents) =>
+      StringSeqToSexpr(["Expression.DatatypeValue",
+                          DatatypeTypeToSexpr(datatypeType),
+                          MapJoin(TypeToSexpr, typeArgs),
+                          NameToSexpr(variant),
+                          Std.Strings.OfBool(isCo),
+                          assert forall x :: x in contents ==> x.1 < expr;
+                          MapJoin(x requires x in contents => TwoTupleToSexpr(x, y => y, (z) requires z < expr => ExpressionToSexpr(z)), contents)])
+    case Convert(value, from, typ) => "TODO"
+    case SeqConstruct(length, elem) => "TODO"
+    case SeqValue(elements, typ) => "TODO"
+    case SetValue(elements) => "TODO"
+    case MultisetValue(elements) => "TODO"
+    case MapValue(mapElems) => "TODO"
+    case MapBuilder(keyType, valueType) => "TODO"
+    case SeqUpdate(expr, indexExpr, value) => "TODO"
+    case MapUpdate(expr, indexExpr, value) => "TODO"
+    case SetBuilder(elemType) => "TODO"
+    case ToMultiset(expr) => "TODO"
+    case This() => "TODO"
+    case Ite(cond, thn, els) => "TODO"
+    case UnOp(unOp, expr, format1) => "TODO"
+    case BinOp(op, left, right, format2) => "TODO"
+    case ArrayLen(expr, dim) => "TODO"
+    case MapKeys(expr) => "TODO"
+    case MapValues(expr) => "TODO"
+    case Select(expr, field, isConstant, onDatatype, fieldType) => "TODO"
+    case SelectFn(expr, field, onDatatype, isStatic, arity) => "TODO"
+    case Index(expr, collKind, indices) => "TODO"
+    case IndexRange(expr, isArray, low, high) => "TODO"
+    case TupleSelect(expr, index, fieldType) => "TODO"
+    case Call(on, callName, typeArgs, args) => "TODO"
+    case Lambda(params, retType, body) => "TODO"
+    case BetaRedex(values, retType, expr) => "TODO"
+    case IIFE(name, typ, value, iifeBody) => "TODO"
+    case Apply(expr, args) => "TODO"
+    case TypeTest(on, dType, variant) => "TODO"
+    case InitializationValue(typ) => "TODO"
+    case BoolBoundedPool() => "TODO"
+    case SetBoundedPool(of) => "TODO"
+    case SeqBoundedPool(of, includeDuplicates) => "TODO"
+    case IntRange(lo, hi) => "TODO"
+  }
+
+  // analogously to TypeToSexpr case
+  function MapJoinExpressionToSexpr(ts: seq<DAST.Expression>): string
+  {
+    MapJoin((x) requires x in ts => (ExpressionToSexpr(x)), ts)
   }
 
   function StatementToSexpr(stmt: DAST.Statement): string {
@@ -151,15 +275,36 @@ module {:extern} DafnyToSExpressionCompiler {
     "TypeArgBoundToSexpr: TODO"
   }
 
+  function FormalToSexpr(formal: DAST.Formal): string {
+    "FormalToSexpr: TODO"
+  }
+
   function ResolvedTypeToSexpr(resolvedType: DAST.ResolvedType): string {
     match resolvedType
     case Datatype(datatypeType) => "ResolvedType.Datatype: TODO"
     case Trait(path, attributes) => "ResolvedType.Trait: TODO"
     case Newtype(baseType, range, erase, attributes) =>
       var mutual_test := TypeToSexpr(baseType);
-    "ResolvedType.Newtype: TODO"
+      "ResolvedType.Newtype: TODO"
   }
 
+  function PrimitiveToSexpr(primitive: DAST.Primitive): string {
+    "PrimitiveToSexpr: TODO"
+  }
+
+  function MethodToSexpr(m: DAST.Method): string {
+    "MethodToSexpr: TODO"
+  }
+
+  function LiteralToSexpr(literal: DAST.Literal): string {
+    "LiteralToSexpr: TODO"
+  }
+
+  function DatatypeTypeToSexpr(datatypeType: DAST.DatatypeType): string {
+    "DatatypeTypeToSexpr: TODO"
+  }
+
+  // Using -> is easier than ~>
   function OptionToSexpr<T>(opt: Std.Wrappers.Option<T>, convert: (T -> string)): string {
     match opt
     case None => "(None)"
@@ -176,6 +321,15 @@ module {:extern} DafnyToSExpressionCompiler {
   // Note that xs is a sequence of strings in Dafny, not DAST.
   function StringSeqToSexpr(xs: seq<string>): string {
     MapJoin(x => x, xs)
+  }
+
+  function TwoTupleToSexpr<T, U>(tuple: (T, U), Tf: (T ~> string), Uf: (U ~> string)): string
+    requires Tf.requires(tuple.0)
+    requires Uf.requires(tuple.1)
+    reads Tf.reads(tuple.0)
+    reads Uf.reads(tuple.1)
+  {
+    StringSeqToSexpr([Tf(tuple.0), Uf(tuple.1)])
   }
 
 }
